src/theories/Config.v
@@ -49,20 +49,14 @@ Definition make_interp_branch (r: term) : branch term :=  {|
   bbody := r
 |}.
 
-Fixpoint tm_make_interp_branches (xs: list Type) (ys: list Set) : TemplateMonad (list (branch term)) := 
+Definition packed_ty := {T & T}.
+
+Fixpoint tm_make_interp_branches (xs: list packed_ty) : TemplateMonad (list (branch term)) := 
   match xs with 
-  | nil => (fix rec ys := 
-      match ys with 
-      | nil => tmReturn nil
-      | y :: ys' => 
-        t <- tmQuote y ;;
-        r <- rec ys' ;;
-        tmReturn (make_interp_branch t :: r)
-      end
-    ) ys
-  | x :: xs' => 
+  | nil => tmReturn nil
+  | (existT _ x) :: xs' => 
     t <- tmQuote x ;;
-    r <- tm_make_interp_branches xs' ys ;;
+    r <- tm_make_interp_branches xs' ;;
     tmReturn (make_interp_branch t :: r)
   end.
 
@@ -77,9 +71,9 @@ Definition quote_dest_ind (t: Type) :=
   end.
 
 
-Definition add_interp_sorts (tys: list Type) (sets: list Set) (sorts: Type) := 
+Definition add_interp_sorts (tys: list packed_ty) (sorts: Type) := 
   '(sort_term, ind) <- quote_dest_ind sorts ;;
-  brs <- tm_make_interp_branches tys sets ;;
+  brs <- tm_make_interp_branches tys ;;
   tmMkDefinition "interp_sorts" (tLambda 
     (mkBindAnn (nNamed "srt") Relevant)
     sort_term
@@ -99,7 +93,6 @@ Definition add_interp_sorts (tys: list Type) (sets: list Set) (sorts: Type) :=
   ).
 
 MetaCoq Quote Definition term_nat := nat.
-
 MetaCoq Quote Definition term_0 := 0.
 
 (* Inductive fin : nat -> Set := f0 : fin 0. *)
@@ -160,8 +153,87 @@ Definition funs_body (funs_arg_term : term) (funs_ret_term: term) (indices: list
   ind_variance := None;
 |}.
 
-Definition add_funs_type (sorts: Type) (indices : list (list term)) := 
+Locate kername.
+
+Definition get_typ (x: global_decl) := 
+  match x with 
+  | ConstantDecl body => body.(cst_type)
+  | InductiveDecl mind => hole
+  end.
+
+Fixpoint normalize_sort_term (t: term) : list term := 
+  match t with 
+  | tProd _ ty bod => normalize_sort_term ty ++ normalize_sort_term bod
+  | tInd _ _ => [t] 
+  | tVar _ => [t]
+  | tApp l rs => 
+    normalize_sort_term l ++ concat (map normalize_sort_term rs)
+  | _ => []
+  end.
+
+Require Import MirrorSolve.Utils.
+Import KernameComp.
+Definition kername_eqb l r :=
+  match compare l r with 
+  | Eq => true
+  | _ => false
+  end.
+
+Definition eq_kname : kername := (MPfile ["Logic"; "Init"; "Coq"], "eq").
+Definition pos_kname : kername := (MPfile ["BinNums"; "Numbers"; "Coq"], "positive").
+
+Definition should_filter (k: kername) := inb _ kername_eqb k [eq_kname; pos_kname].
+
+Fixpoint get_sorts' ( decls: global_declarations ) : list term := 
+  match decls with 
+  | nil => nil
+  | (kn, decl) :: decls' => 
+    let r := get_sorts' decls' in 
+      if should_filter kn then r else 
+      match decl with 
+      | ConstantDecl cd => normalize_sort_term cd.(cst_type) ++ r
+      | _ => r
+      end
+  end.
+
+Require MirrorSolve.Reflection.Core.
+
+Definition get_sorts decls := uniq _ Core.eq_term (get_sorts' decls).
+
+Fixpoint quote_indices (sorts: Type) (indices : list (list sorts * sorts)) : TemplateMonad (list (list term)) :=
+  match indices with 
+  | nil => tmReturn nil
+  | (args, ret) :: indices' => 
+    args_term <- tmQuote args ;;
+    ret_term <- tmQuote ret ;;
+    r <- quote_indices _ indices' ;;
+    tmReturn ([args_term; ret_term] :: r)
+  end.
+
+Definition add_funs_type (sorts: Type) (indices : list (list sorts * sorts)) : TemplateMonad unit := 
   arg_term <- tmQuote (list sorts) ;;
   ret_term <- tmQuote sorts ;;
   funs_ty_term <- tmQuote (list sorts -> sorts -> Type) ;;
-  tmMkInductive' (funs_body arg_term ret_term indices funs_ty_term).
+  indices' <- quote_indices sorts indices ;;
+  tmMkInductive' (funs_body arg_term ret_term indices' funs_ty_term).
+
+
+Definition make_names (prefix: ident) (xs: list term) : list ident := 
+  map_with_index (fun i _ => prefix ++ "_" ++ (String.of_string (n_to_str i))) xs.
+
+Definition uniq_term := uniq _ Core.eq_term.
+
+
+(* TODO: 
+  1) add a new sort interpretation, unquoting sort_ty_terms to get the types
+  2) add function symbols, using the new sort and the indices as constructor arguments
+  
+*)
+Definition add_funs_indices (indices: list (list term)) := 
+  let sort_ty_terms := uniq_term (concat indices) in 
+  let sort_names := make_names "srt" sort_ty_terms in 
+  add_sorts sort_names.
+
+
+(* MetaCoq Run (add_funs_indices [[tRel 0; tRel 1]]). *)
+
